finish the proof of pstore_2

theories/persistent/pstore_2.v
@@ -37,6 +37,9 @@ Implicit Types σ : gmap loc val.
 ( in custom zebre_tag
 ).
 
+(* ------------------------------------------------------------------------ *)
+(* The code *)
+
 Definition pstore_create : val :=
   λ: <>,
     ref (ref §Root).
@@ -120,60 +123,65 @@ Qed.
 
 #[local] Existing Instance pstore_G_map_G.
 
-(* Define [rtcl]: a rtc in a labeled transition system. *)
-Section rtc_lab.
-Context {A B:Type}.
-Context (R:A -> B -> A -> Prop).
+(* ------------------------------------------------------------------------ *)
+(* More lemmas on maps and lists *)
+Section more_map.
+  Context `{Countable K}.
+  Context {V:Type}.
 
-Inductive rtcl : A -> list B -> A -> Prop :=
-| rtcl_refl : forall a, rtcl a [] a
-| rtcl_l : forall a1 b a2 bs a3,
-    R a1 b a2 ->
-    rtcl a2 bs a3 ->
-    rtcl a1 (b::bs) a3.
+  Lemma gmap_included_insert (σ1 σ2:gmap K V) (l:K) (v:V) :
+    σ1 ⊆ σ2 ->
+    <[l:=v]>σ1 ⊆ <[l:=v]>σ2.
+  Proof.
+    intros ? l'. destruct_decide (decide (l=l')).
+    { subst. rewrite !lookup_insert //. }
+    { rewrite !lookup_insert_ne //. }
+  Qed.
 
-Lemma rtcl_r a1 b a2 bs a3 :
-  rtcl a1 bs a2 ->
-  R a2 b a3 ->
-  rtcl a1 (bs++[b]) a3.
-Proof.
-  induction 1.
-  { eauto using rtcl_refl,rtcl_l. }
-  { intros. rewrite -app_comm_cons. eauto using rtcl_l. }
-Qed.
+  Lemma gmap_included_insert_notin (σ1 σ2:gmap K V) (l:K) (v:V) :
+    l ∉ dom σ1 ->
+    σ1 ⊆ σ2 ->
+    σ1 ⊆ <[l:=v]>σ2.
+  Proof.
+    intros ?? l'. destruct_decide (decide (l=l')).
+    { subst. rewrite lookup_insert // not_elem_of_dom_1 //. }
+    { rewrite !lookup_insert_ne //. }
+  Qed.
 
+  Lemma incl_dom_incl (σ1 σ2:gmap K V)  :
+    σ1 ⊆ σ2 ->
+    dom σ1 ⊆ dom σ2.
+  Proof.
+    intros X1.
+    intros l Hl. apply elem_of_dom in Hl. destruct Hl as (?&Hl).
+    eapply map_subseteq_spec in X1; last done. by eapply elem_of_dom.
+  Qed.
+End more_map.
 
-Lemma rtcl_ind_r_weak (P : A -> list B → A → Prop)
-  (Prefl : ∀ x, P x [] x) (Pstep : ∀ x bs y b z, rtcl x bs y → R y b z → P x bs y → P x (bs++[b]) z) :
-  ∀ x bs z, rtcl x bs z → P x bs z.
-Proof.
-  cut (∀ y bs z, rtcl y bs z → ∀ x bs', rtcl x bs' y → P x bs' y → P x (bs'++bs) z).
-  { intros. specialize (H x bs z H0 x nil). simpl in *. eauto using rtcl_refl. }
-  { induction 1.
-    { intros. rewrite right_id_L //. }
-    { intros. rewrite cons_middle assoc_L. eauto using rtcl_r. } }
-Qed.
+Section more_list.
+  Context {A:Type}.
 
-Lemma rtcl_ind_r (P : list B -> A → Prop) (x : A)
-  (Prefl : P nil x) (Pstep : ∀ bs y b z, rtcl x bs y → R y b z → P bs y → P (bs++[b]) z) :
-  ∀ bs z, rtcl x bs z → P bs z.
-Proof.
-  intros bs z p. revert x bs z p Prefl Pstep.
-  refine (rtcl_ind_r_weak _ _ _); eauto.
-Qed.
+  Lemma list_case_r (l:list A) :
+    l = nil \/ exists (l':list A) x, l = l' ++ [x].
+  Proof.
+    induction l using rev_ind.
+    naive_solver. right.
+    destruct IHl as [-> | (?&?&->)]; eauto.
+  Qed.
 
-Lemma rtcl_inv_r x bs z :
-  rtcl x bs z → (x = z /\ bs = nil) ∨ ∃ bs' b y, bs = bs' ++ [b] /\ rtcl x bs' y ∧ R y b z.
-Proof.
-  revert bs z. apply rtcl_ind_r; eauto.
-  intros ?????? [(->&->)|(bs'&b&y&->&?&?)]; right.
-  { exists nil. eauto using rtcl_refl. }
-  { exists (bs' ++ [b]). eauto. }
-Qed.
+  Lemma elem_of_middle (x:A) (xs:list A) :
+    x ∈ xs ->
+    exists (l1 l2:list A), xs = l1 ++ x::l2.
+  Proof.
+    intros Hx. apply elem_of_list_lookup_1 in Hx.
+    destruct Hx as (?&?).
+    eexists _,_. symmetry. eapply take_drop_middle. done.
+  Qed.
+End more_list.
 
-End rtc_lab.
-
+(* ------------------------------------------------------------------------ *)
 (* Define a labeled graph, as a set of edges. *)
+
 Section Graph.
 Definition graph (A B:Type) `{Countable A} `{Countable B} := gset (A*B*A).
 
@@ -185,8 +193,12 @@ Lemma vertices_empty :
   vertices ∅ = ∅.
 Proof. compute_done. Qed.
 
-Definition vin {A B C:Type} (x:(A*B*C)) := match x with (a,_,_) => a end.
-Definition vout {A B C:Type} (x:(A*B*C)) := match x with (_,_,c) => c end.
+Definition proj1 {A B C:Type} (x:(A*B*C)) : A :=
+  match x with (x,_,_) => x end.
+Definition proj2 {A B C:Type} (x:(A*B*C)) : B :=
+  match x with (_,x,_) => x end.
+Definition proj3 {A B C:Type} (x:(A*B*C)) : C :=
+  match x with (_,_,x) => x end.
 
 Lemma elem_of_vertices x (g:graph A B) :
   x ∈ vertices g <-> exists b y, ((x,b,y) ∈ g \/ (y,b,x) ∈ g).
@@ -197,7 +209,7 @@ Proof.
 Qed.
 
 Lemma vertices_singleton (x:(A*B*A)) :
-  vertices {[x]} = {[vin x; vout x]}.
+  vertices {[x]} = {[proj1 x; proj3 x]}.
 Proof.
   rewrite /vertices set_fold_singleton. destruct x as ((?&?)&?); set_solver.
 Qed.
@@ -213,7 +225,7 @@ Proof.
   destruct_decide (decide (x ∈ g2)).
   { replace ({[x]} ∪ g2) with g2 by set_solver.
     rewrite vertices_singleton.
-    assert ({[vin x; vout x]} ⊆ vertices g2); last by set_solver.
+    assert ({[proj1 x; proj3 x]} ⊆ vertices g2); last by set_solver.
     intros l Hl. apply elem_of_vertices.
     rewrite elem_of_union !elem_of_singleton in Hl. destruct x as ((?,?),?). set_solver. }
   rewrite {1}/vertices /set_fold. simpl.
@@ -223,74 +235,7 @@ Proof.
   { simpl. rewrite vertices_singleton. destruct x as ((?,?),?). set_solver. }
 Qed.
 
-
 Definition edge (g:graph A B) x c y := (x,c,y) ∈ g.
-Definition reachable (g:graph A B) x bs y := rtcl (edge g) x bs y.
-
-Lemma reachable_weak g1 g2 x bs y :
-  reachable g1 x bs y ->
-  g1 ⊆ g2 ->
-  reachable g2 x bs y.
-Proof.
-  induction 1; intros Hi. apply rtcl_refl. eapply rtcl_l.
-  by apply Hi. by apply IHrtcl.
-Qed.
-
-Lemma reachable_inv_in_invertices g x1 ds x2 :
-  reachable g x1 ds x2 ->
-  (x1 = x2) \/ (x1 ∈ vertices g /\ x2 ∈ vertices g).
-Proof.
-  inversion 1. eauto. subst. right.
-  split. apply elem_of_vertices. eauto.
-  apply rtcl_inv_r in H3. destruct H3 as [(->&->)|(?&?&?&->&?&?)].
-  all:apply elem_of_vertices; eauto.
-Qed.
-
-Lemma reachable_cycle_end_inv_aux g (r r':A) b ds x1 x2 :
-  r ≠ r' ->
-  x2 ≠ r' ->
-  r' ∉ vertices g ->
-  reachable ({[(r, b, r')]} ∪ g) x1 ds x2 ->
-  reachable g x1 ds x2.
-Proof.
-  induction 4.
-  { apply rtcl_refl. }
-  { eapply rtcl_l with a2.
-    { rewrite /edge elem_of_union elem_of_singleton in H4.
-      destruct H4 as [|]; last done.
-      inversion H4. subst. inversion H5. congruence. subst.
-      exfalso. apply H3. apply elem_of_vertices. set_solver. }
-    by eapply IHrtcl. }
-Qed.
-
-Lemma reachable_cycle_end_inv g (r r':A) b ds x :
-  r ≠ r' ->
-  r' ∉ vertices g ->
-  reachable ({[(r, b, r')]} ∪ g) x ds x ->
-  reachable g x ds x.
-Proof.
-  intros.
-  destruct_decide (decide (x=r')).
-  { subst. inversion H3. apply rtcl_refl. subst. exfalso. apply H2. apply elem_of_vertices. set_solver. }
-  eapply reachable_cycle_end_inv_aux; last done. all:done.
-Qed.
-
-Lemma reachable_add_end (r r':A) b x ds g :
-  r ≠ r' ->
-  r' ∉ vertices g ->
-  reachable ({[(r, b, r')]} ∪ g) x ds r' ->
-  (ds = nil /\ x = r') \/ (exists ds', ds = ds' ++ [b] /\ reachable g x ds' r).
-Proof.
-  intros Hrr' Hr' Hreach. apply rtcl_inv_r in Hreach.
-  destruct Hreach as [(->&->)|(bs'&b0&y&->&Hreach&Hedge)].
-  { eauto. }
-  right.
-  assert (b0=b /\ y=r) as (->&->).
-  { rewrite /edge elem_of_union elem_of_singleton in Hedge.
-    destruct Hedge. naive_solver. exfalso. apply Hr', elem_of_vertices. eauto. }
-  eexists. split; first done.
-  eauto using reachable_cycle_end_inv_aux.
-Qed.
 
 Inductive path (g:graph A B) : A -> list (A*B*A) -> A -> Prop :=
 | path_nil : forall a, path g a [] a
@@ -298,34 +243,6 @@ Inductive path (g:graph A B) : A -> list (A*B*A) -> A -> Prop :=
     (a1,b,a2) ∈ g ->
     path g a2 bs a3 ->
     path g a1 ((a1,b,a2)::bs) a3.
-
-Definition proj1 {A B C:Type} (x:(A*B*C)) : A :=
-  match x with (x,_,_) => x end.
-Definition proj2 {A B C:Type} (x:(A*B*C)) : B :=
-  match x with (_,x,_) => x end.
-Definition proj3 {A B C:Type} (x:(A*B*C)) : C :=
-  match x with (_,_,x) => x end.
-
-Lemma reachable_path g a1 a2 ds :
-  reachable g a1 ds a2 ->
-  exists xs, path g a1 xs a2 /\ (proj2 <$> xs = ds).
-Proof.
-  intros Hreach. induction Hreach.
-  { exists nil. split_and !; try done. eauto using path_nil. }
-  { destruct IHHreach as (xs&?&Hxs).
-    exists ((a1,b,a2)::xs). split_and !.
-    { eauto using path_cons. }
-    { set_solver. } }
-Qed.
-
-Lemma reachable_path2 g a1 a2 xs :
-  path g a1 xs a2 ->
-  reachable g a1 (proj2 <$> xs) a2.
-Proof.
-  induction 1.
-  { intros. apply rtcl_refl. }
-  { apply rtcl_l with a2. set_solver. done. }
-Qed.
 
 Lemma path_app_inv g a1 a2 xs ys :
   path g a1 (xs ++ ys) a2 ->
@@ -352,6 +269,65 @@ Record rooted_dag g (r:A) :=
   { ti1 : forall a, a ∈ vertices g -> exists xs, path g a xs r;
     ti2 : acyclic g
   }.
+
+Definition unaliased (g:graph A B) :=
+    forall r x1 r1 x2 r2,
+    (r,x1,r1) ∈ g ->
+    (r,x2,r2) ∈ g ->
+    x1 = x2 /\ r1 = r2.
+
+Lemma path_app (g:graph A B) x3 x1 xs ys x2 :
+  path g x1 xs x3 ->
+  path g x3 ys x2 ->
+  path g x1 (xs++ys) x2.
+Proof.
+  intros Hp.
+  revert x2 ys. induction Hp. eauto.
+  intros. rewrite -app_comm_cons. apply path_cons. set_solver.
+  eauto.
+Qed.
+
+Definition all_uniq_path g :=
+  forall a1 a2 xs ys, path g a1 xs a2 -> path g a1 ys a2 -> xs = ys.
+
+Lemma rooted_tree_impl_acyclic_unaliased g r :
+  (forall a, a ∈ vertices g -> exists xs, path g a xs r) -> (* If every vertex can reach the root, *)
+  all_uniq_path g -> (* then the property of uniq path *)
+  acyclic g /\ unaliased g. (* implies acyclicity + unalising *)
+Proof.
+  intros Hroot  Huniq. split.
+  { intros ?? Hpath.
+    assert (path g a (xs++xs) a) as Hloop.
+    { by eapply path_app. }
+    specialize (Huniq a a xs (xs++xs) Hpath Hloop).
+    apply (@f_equal _ _ length) in Huniq. rewrite app_length in Huniq.
+    assert (length xs = 0) by lia. destruct xs; simpl in *; try done; lia. }
+  { intros ????? X1 X2.
+    destruct (Hroot r1) as (xs1&Hxs1).
+    { eapply elem_of_vertices. eauto. }
+    destruct (Hroot r2) as (xs2&Hxs2).
+    { eapply elem_of_vertices. eauto. }
+    assert (path g r0 ((r0,x1,r1)::xs1) r) as Hp1. by eapply path_cons.
+    assert (path g r0 ((r0,x2,r2)::xs2) r) as Hp2. by eapply path_cons.
+    specialize (Huniq _ _ _ _ Hp1 Hp2). naive_solver. }
+Qed.
+
+Lemma acyclic_unaliased_impl_uniq_path g :
+  acyclic g ->
+  unaliased g ->
+  all_uniq_path g.
+Proof.
+  intros Hacy Hinj. intros ???? Hpath.
+  revert ys. induction Hpath; intros ys.
+  { intros Hpath. apply Hacy in Hpath. done. }
+  { inversion 1; subst.
+    { exfalso.
+      assert (path g a3 ((a3, b, a2)::bs) a3) as Z.
+      { apply path_cons. done. eauto. }
+      apply Hacy in Z. congruence. }
+    destruct (Hinj _ _ _ _ _ H1 H3). subst.
+    f_equal. eapply IHHpath. done. }
+Qed.
 
 Lemma rooted_dag_empty (r:A) :
     rooted_dag (∅ : graph A B) r.
@@ -390,7 +366,7 @@ Proof.
   eapply path_cycle_end_inv_aux; last done. all:done.
 Qed.
 
-Lemma path_r g a1 b a2 bs a3 :
+Lemma path_snoc g a1 b a2 bs a3 :
   path g a1 bs a2 ->
   (a2,b,a3) ∈ g ->
   path g a1 (bs++[(a2,b,a3)]) a3.
@@ -409,43 +385,6 @@ Proof.
   by apply Hi. by apply IHpath.
 Qed.
 
-Definition kindofinj (g:graph A B) :=
-    forall r x1 r1 x2 r2,
-    (r,x1,r1) ∈ g ->
-    (r,x2,r2) ∈ g ->
-    x1 = x2 /\ r1 = r2.
-
-Lemma use_kindofinj g a1 xs ys a2 :
-  acyclic g ->
-  kindofinj g ->
-  path g a1 xs a2 ->
-  path g a1 ys a2 ->
-  xs = ys.
-Proof.
-  intros Hacy Hinj Hpath. revert ys. induction Hpath; intros ys.
-  { intros Hpath. apply Hacy in Hpath. done. }
-  { inversion 1; subst.
-    { exfalso.
-      assert (path g a3 ((a3, b, a2)::bs) a3) as Z.
-      { apply path_cons. done. eauto. }
-      apply Hacy in Z. congruence. }
-    destruct (Hinj _ _ _ _ _ H1 H3). subst.
-    f_equal. eapply IHHpath. done. }
-Qed.
-
-Lemma rooted_dag_root_no_succ g r x r' :
-  rooted_dag g r ->
-  (r,x,r') ∉ g.
-Proof.
-  intros [X1 X2] Hg.
-  assert (r' ∈ vertices g) as E4.
-  { apply elem_of_vertices. set_solver. }
-  apply X1 in E4. destruct E4 as (zs&?).
-  assert (path g r ((r, x, r')::zs) r) as Hpath.
-  { apply path_cons. set_solver. done. }
-  eapply X2 in Hpath. congruence.
-Qed.
-
 Lemma rooted_dag_add (r r':A) g x:
   r ≠ r' ->
   r' ∉ vertices g ->
@@ -460,154 +399,208 @@ Proof.
     { exists [(r, x, r')]. simpl. eapply path_cons. set_solver. apply path_nil. }
     { exists nil. apply path_nil. }
     { apply X1 in Hx. destruct Hx as (ds,Hx). exists (ds++[(r, x, r')]).
-      eapply path_r.
+      eapply path_snoc.
       { eapply path_weak; eauto. set_solver. }
       { set_solver. } } }
   { intros ?? Hpath. apply  path_cycle_end_inv in Hpath; eauto. }
 Qed.
+
+Lemma acyclic_weak (g1 g2:graph A B) :
+  acyclic g1 ->
+  g2 ⊆ g1 ->
+  acyclic g2.
+Proof.
+  intros Hacy ? ???. eapply Hacy. by eapply path_weak.
+Qed.
+
+Lemma path_all_in (g:graph A B) a1 xs a2 :
+  path g a1 xs a2 ->
+  list_to_set xs ⊆ g.
+Proof.
+  induction 1; simpl; set_solver.
+Qed.
+
+Lemma path_restrict (g:graph A B) r xs r' :
+  path g r xs r' ->
+  path (list_to_set xs) r xs r'.
+Proof.
+  induction 1; eauto using path_nil.
+  apply path_cons. set_solver.
+  eapply path_weak. done. set_solver.
+Qed.
+
+Lemma path_inv_r (g:graph A B) x bs z :
+  path g x bs z ->
+  (x = z /\ bs = nil) ∨ ∃ bs' b y, bs = bs' ++ [(y,b,z)] /\ path g x bs' y ∧ (y,b,z) ∈ g.
+Proof.
+  induction 1.
+  { naive_solver.  }
+  right. destruct IHpath as [(->&->)|(bs'&b'&y&->&?&?)].
+  { exists nil. eexists _,_. split; first done. split. eauto using path_nil. naive_solver. }
+  { exists ((a1, b, a2) :: bs'). eexists _,_. rewrite app_comm_cons //. split_and !; try done.
+    apply path_cons; eauto. }
+Qed.
+
+Lemma path_add_inv_r (r r':A) b x xs g :
+  r ≠ r' ->
+  r' ∉ vertices g ->
+  path ({[(r, b, r')]} ∪ g) x xs r' ->
+  (xs = nil /\ x = r') \/ (exists xs', xs = xs' ++ [(r, b, r')] /\ path g x xs' r).
+Proof.
+  intros Hrr' Hr' Hreach. apply path_inv_r in Hreach.
+  destruct Hreach as [(->&->)|(bs'&b0&y&->&Hreach&Hedge)].
+  { eauto. }
+  right.
+  assert (b0=b /\ y=r) as (->&->).
+  { rewrite /edge elem_of_union elem_of_singleton in Hedge.
+    destruct Hedge. naive_solver. exfalso. apply Hr', elem_of_vertices. eauto. }
+  eexists. split; first done.
+  eauto using path_cycle_end_inv_aux.
+Qed.
+
+(* [mirror xs ys] asserts that, up-to labels, the path xs is the reverse of ys *)
+Inductive mirror :
+  list (A*B*A) -> list (A*B*A) -> Prop :=
+| mirror_nil :
+  mirror [] []
+| mirror_cons :
+  forall r x x' r' xs ys,
+    mirror xs ys  ->
+    mirror (xs++[(r,x,r')]) ((r',x',r)::ys).
+
+Lemma mirror_snoc ys xs a a' x x' :
+  mirror ys xs ->
+  mirror ((a,x,a') :: ys) (xs ++ [(a',x',a)]).
+Proof.
+  induction 1.
+  { apply (mirror_cons _ _ _ _ nil nil). apply mirror_nil. }
+  rewrite -!app_comm_cons app_comm_cons. by apply mirror_cons.
+Qed.
+
+Lemma mirror_symm xs ys :
+  mirror xs ys -> mirror ys xs.
+Proof.
+  induction 1. eauto using mirror_nil.
+  apply mirror_snoc; eauto.
+Qed.
+
+Lemma use_mirror xs ys (g:graph A B) r y :
+  mirror xs ys ->
+  path g r xs y ->
+  path (list_to_set ys) y ys r.
+Proof.
+  intros Hu. revert r y. induction Hu; intros r0 y.
+  { inversion 1. subst. apply path_nil. }
+  intros Hp. apply path_snoc_inv in Hp. destruct Hp as (?&?&?). subst.
+  apply path_cons. set_solver. eapply path_weak. apply IHHu; eauto. set_solver.
+Qed.
+
+Lemma mirror_vertices (xs ys:list (A*B*A)) :
+  mirror xs ys ->
+  vertices (list_to_set ys) = vertices (list_to_set xs).
+Proof.
+  revert xs. induction ys; intros xs; inversion 1; subst. done.
+  simpl. rewrite list_to_set_app_L !vertices_union !vertices_singleton. simpl.
+  erewrite IHys; last done. rewrite vertices_empty. set_solver.
+Qed.
+
+Lemma mirror_same_length (xs ys:list (A*B*A)):
+  mirror xs ys ->
+  length xs = length ys.
+Proof. induction 1. done. rewrite app_length. simpl. lia. Qed.
+
+Lemma mirror_mirrored_edges xs ys r x r' :
+  mirror xs ys ->
+  (r,x,r') ∈ xs -> exists x', (r',x',r) ∈ ys.
+Proof.
+  induction 1. intros ?. set_solver.
+  rewrite elem_of_app elem_of_list_singleton.
+  intros [X|X].
+  { apply IHmirror in X. set_solver. }
+  { set_solver. }
+Qed.
+
+Lemma path_middle (g:graph A B) x xs ys z :
+  path g x (xs ++ ys) z ->
+  exists y, path g x xs y /\ path g y ys z.
+Proof.
+  revert g x ys z. induction xs; intros g x ys z.
+  { simpl. eauto using path_nil. }
+  inversion 1; simpl in *; subst.
+  apply IHxs in H7. destruct H7 as (y,(?&?)).
+  exists y. split; last done. eauto using path_cons.
+Qed.
+
+Lemma use_mirror_subset xs ys xs' g r y :
+  xs' ⊆ xs ->
+  mirror xs ys ->
+  path g r xs' y ->
+  exists zs, path (list_to_set ys) y zs r /\ length xs' = length zs.
+Proof.
+  intros Hincl Hundo Hpath.
+  induction Hpath.
+  { exists nil. split. apply path_nil. done. }
+  { destruct IHHpath as (zs&Hzs&?).
+    { set_solver. }
+    eapply (mirror_mirrored_edges _ _ a1 b a2) in Hundo. 2:set_solver.
+    destruct Hundo as (b'&?).
+    exists (zs ++ [(a2, b', a1)]). split.
+    { eapply path_app. done.
+      apply path_cons.  set_solver. apply path_nil. }
+    { rewrite app_length. simpl. lia. } }
+Qed.
+
+Definition pathlike (ys:list (A*B*A)) r :=
+  forall a b a', (a,b,a') ∈ ys -> a' = r \/ exists b' a'', (a',b',a'') ∈ ys.
+
+Lemma path_pathlike g r ys y :
+  path g y ys r ->
+  pathlike ys r.
+Proof.
+  intros Hpath a b a' Hedge.
+  apply elem_of_middle in Hedge. destruct Hedge as (?&?&->).
+  rewrite cons_middle assoc_L in Hpath.
+  apply path_app_inv in Hpath. destruct Hpath as (?&Hpath&Hp').
+  apply path_snoc_inv in Hpath. destruct Hpath as (?&?&?). subst.
+  inversion Hp'; set_solver.
+Qed.
+
+Lemma same_path g (xs:list (A*B*A)) a1 a2 a3 a4 :
+  path g a1 xs a2 ->
+  path g a3 xs a4 ->
+  xs ≠ nil ->
+  a1 = a3 /\ a2=a4.
+Proof.
+  intros Hp1. revert a3 a4. induction Hp1.
+  { intros. congruence. }
+  intros a3' a4'. inversion 1. subst. intros _. destruct bs.
+  { inversion Hp1; inversion H10. subst. done. }
+  apply IHHp1 in H10. 2:done. naive_solver.
+Qed.
+
+Lemma path_ends_vertices g x1 xs x2 :
+  path g x1 xs x2 ->
+  (x1 = x2) \/ (x1 ∈ vertices g /\ x2 ∈ vertices g).
+Proof.
+   inversion 1. eauto. subst. right.
+   split. apply elem_of_vertices. eauto.
+   apply path_inv_r in H3. destruct H3 as [(->&->)|(?&?&?&->&?&?)].
+   all:apply elem_of_vertices; eauto.
+Qed.
+
 End Graph.
 
-Section pstore_G.
-  Context `{pstore_G : PstoreG Σ}.
-
+(* ------------------------------------------------------------------------ *)
+(* Define apply_diffl, a function applying a list of diff. *)
+Section adiffl.
   Notation diff := (loc*val)%type. (* the loc and its old value. *)
-  Notation graph_store := (graph loc diff).
-  Notation map_model := (gmap loc (gmap loc val)).
 
   Definition apply_diffl (ds:list diff) (σ:gmap loc val) : gmap loc val :=
     foldr (fun '(l,v) σ => <[l:=v]> σ) σ ds.
 
-  Record store_inv (M:map_model) (g:graph_store) (r:loc) (σ σr:gmap loc val) :=
-    { si1 : dom M = vertices g ∪ {[r]};
-      si2 : σ ⊆ σr;
-      si3 : M !! r = Some σr ;
-      si4 : forall r1 ds r2 σ1 σ2,
-        reachable g r1 ds r2 -> M !! r1 = Some σ1 -> M !! r2 = Some σ2 -> σ1 ⊆ (apply_diffl ds σ2)
-    }.
-
-  Definition locs_of_edges_in g (X:gset loc) :=
-    forall (r:loc) l v r', edge g r (l,v) r' -> l ∈ X.
-
-  Record coherent (σ0 σr:gmap loc val) (g:graph_store) :=
-    { coh1 : σr ⊆ σ0;
-      coh2 : locs_of_edges_in g (dom σ0);
-    }.
-
-
-  Lemma gmap_included_insert `{Countable K} {V} (σ1 σ2:gmap K V) (l:K) (v:V) :
-    σ1 ⊆ σ2 ->
-    <[l:=v]>σ1 ⊆ <[l:=v]>σ2.
-  Proof.
-    intros ? l'. destruct_decide (decide (l=l')).
-    { subst. rewrite !lookup_insert //. }
-    { rewrite !lookup_insert_ne //. }
-  Qed.
-
-  Lemma gmap_included_insert_notin `{Countable K} {V} (σ1 σ2:gmap K V) (l:K) (v:V) :
-    l ∉ dom σ1 ->
-    σ1 ⊆ σ2 ->
-    σ1 ⊆ <[l:=v]>σ2.
-  Proof.
-    intros ?? l'. destruct_decide (decide (l=l')).
-    { subst. rewrite lookup_insert // not_elem_of_dom_1 //. }
-    { rewrite !lookup_insert_ne //. }
-  Qed.
-
-  Lemma incl_dom_incl σ0 σ  :
-    σ ⊆ σ0 ->
-    dom σ ⊆ dom σ0.
-  Proof.
-    intros X1.
-    intros l Hl. apply elem_of_dom in Hl. destruct Hl as (?&Hl).
-    eapply map_subseteq_spec in X1; last done. by eapply elem_of_dom.
-  Qed.
-
-  Definition snap_inv (M:map_model) (C:gmap nat (loc * gmap loc val)) :=
-    forall n l σ, C !! n = Some (l,σ) -> exists σ', M !! l = Some σ' /\ σ ⊆ σ'.
-
-  #[local] Definition pstore_map_auth γ map :=
-    @map_agree_auth _ _ _ _ _ pstore_G_map_G γ map.
-  #[local] Definition pstore_map_elem γ n l σ :=
-    @map_agree_elem _ _ _ _ _ pstore_G_map_G γ n (l,σ).
-
-  Lemma extract_kindofinj g :
-    ([∗ set] '(r, (l, v), r') ∈ g, r ↦ ’Diff{ #(LiteralLoc l), v, #(LiteralLoc r') }) -∗
-    ⌜kindofinj g⌝.
-  Proof.
-    iIntros "Hg" (???????).
-    destruct_decide (decide (a0 = a2 ∧ a1 = a3)). done.
-    rewrite (big_sepS_delete _ _ (a, a0, a1)). set_solver.
-    rewrite (big_sepS_delete _ _ (a, a2, a3)). set_solver.
-    iDestruct "Hg" as "(?&?&_)". destruct a0,a2.
-    iDestruct (mapsto_ne with "[$][$]") as "%". congruence.
-  Qed.
-
-  (* NB our invariant asserts that g is indeed a rooted tree: a rooted DAG
-     with unicity of paths. Indeed, from the set of pointsto we can extract [kindofinj],
-     (see [extract_kindofinj]), and a DAG with kindofinj guarantees unicity of paths
-     (see [use_kindofinj] ) *)
-
-  #[local] Definition pstore (γ:gname) (t:val) (σ:gmap loc val) : iProp Σ :=
-    ∃ (t0 r:loc) (σ0:gmap loc val) (* the global map, with all the points-to ever allocated *)
-      (σr:gmap loc val) (* The largest model of the root *)
-      (g:graph_store)
-      (M:map_model)
-      (C:gmap nat (loc * gmap loc val)),
-    ⌜t=#t0 /\ store_inv M g r σ σr /\ coherent σ0 σr g /\ rooted_dag g r /\ snap_inv M C⌝ ∗
-    t0 ↦ #(LiteralLoc r) ∗
-    r ↦ §Root ∗
-    pstore_map_auth γ C ∗
-    ([∗ map] l ↦ v ∈ σ0, l ↦ v) ∗
-    ([∗ set] x ∈ g, let '(r,(l,v),r') := x in r ↦ ’Diff{ #(LiteralLoc l), v, #(LiteralLoc r') }) .
-
-  Definition open_inv : string :=
-    "[%t0 [%r [%σ0 [%σr [%g [%M [%C ((->&%Hinv&%Hcoh&%Hgraph&%Hsnap)&Ht0&Hr&HC&Hσ0&Hg)]]]]]]]".
-
-  Lemma pstore_create_spec :
-    {{{ True }}}
-      pstore_create ()
-    {{{ t γ,
-      RET t;
-        pstore γ t ∅
-    }}}.
-  Proof.
-    iIntros "%Φ _ HΦ".
-    wp_rec.
-    wp_alloc r as "Hroot".
-    wp_alloc t0 as "Ht0".
-    iMod (map_agree_alloc ∅) as "[%γ ?]".
-    iApply "HΦ". iModIntro.
-    iExists t0,r,∅,∅,∅,{[r := ∅]},∅. iFrame.
-    rewrite !big_sepM_empty big_sepS_empty !right_id.
-    iPureIntro. split_and!; first done.
-    { constructor.
-      { rewrite dom_singleton_L vertices_empty //. set_solver. }
-      { set_solver. }
-      { rewrite lookup_insert //. }
-      { intros ????? Hr.
-        rewrite !lookup_singleton_Some.
-        inversion Hr; set_solver. } }
-    { constructor. set_solver.
-      { intros ????. set_solver. } }
-    { eauto using rooted_dag_empty. }
-    { intros ??. set_solver. }
-  Qed.
-
-  Lemma use_locs_of_edges_in  g r ds r' X :
-    locs_of_edges_in g X ->
-    reachable g r ds r' ->
-    (list_to_set ds.*1) ⊆ X.
-  Proof.
-    intros He.
-    induction 1. set_solver.
-    apply He in H. set_solver.
-  Qed.
-
   Lemma dom_apply_diffl ds σ :
     dom (apply_diffl ds σ) = dom σ ∪ (list_to_set ds.*1).
-  Proof.
-    induction ds as [|(?&?)]; set_solver.
-  Qed.
+  Proof. induction ds as [|(?&?)]; set_solver. Qed.
 
   Lemma apply_diffl_insert_ne ds l v σ :
     l ∉ ds.*1 ->
@@ -623,6 +616,144 @@ Section pstore_G.
     apply_diffl (ds++ds') σ = apply_diffl ds (apply_diffl ds' σ).
   Proof. rewrite /apply_diffl foldr_app //. Qed.
 
+  Lemma apply_diffl_snoc xs l v σ :
+    apply_diffl (xs ++ [(l,v)]) σ = apply_diffl xs (<[l:=v]> σ).
+  Proof. rewrite apply_diffl_app //. Qed.
+
+  Lemma apply_diffl_cons l v xs σ :
+    apply_diffl ((l,v)::xs) σ = <[l:=v]> (apply_diffl xs σ).
+  Proof. done. Qed.
+
+  Lemma apply_diffl_included xs σ1 σ2 :
+    σ1 ⊆ σ2 ->
+    apply_diffl xs σ1 ⊆ apply_diffl xs σ2.
+  Proof.
+    revert σ1 σ2. induction xs as [|(?,?)]; intros;
+      [ done | eauto using gmap_included_insert ].
+  Qed.
+End adiffl.
+
+(* ------------------------------------------------------------------------ *)
+(* Starting the proof. *)
+Section pstore_G.
+  Context `{pstore_G : PstoreG Σ}.
+
+  Notation diff := (loc*val)%type. (* the loc and its old value. *)
+  Notation graph_store := (graph loc diff).
+  Notation map_model := (gmap loc (gmap loc val)).
+
+  Definition correct_path_diff (M:map_model) (g:graph_store) :=
+    forall r1 ds r2 σ1 σ2,
+      path g r1 ds r2 -> M !! r1 = Some σ1 -> M !! r2 = Some σ2 ->
+      σ1 = (apply_diffl (proj2 <$> ds) σ2).
+
+  Record store_inv (M:map_model) (g:graph_store) (r:loc) (σ σ0:gmap loc val) :=
+    { si1 : dom M = vertices g ∪ {[r]};
+      si2 : σ ⊆ σ0;
+      si3 : M !! r = Some σ0 ;
+      si4 : correct_path_diff M g
+    }.
+
+  Definition locs_of_edges_in g (X:gset loc) :=
+    forall (r:loc) l v r', edge g r (l,v) r' -> l ∈ X.
+
+  Record coherent (M:map_model) (σ0:gmap loc val) (g:graph_store) :=
+    { coh1 : forall r σ, M !! r = Some σ -> dom σ = dom σ0;
+      coh2 : locs_of_edges_in g (dom σ0);
+    }.
+
+  Definition snap_inv (M:map_model) (C:gmap nat (loc * gmap loc val)) :=
+    forall n l σ, C !! n = Some (l,σ) -> exists σ', M !! l = Some σ' /\ σ ⊆ σ'.
+
+  #[local] Definition pstore_map_auth γ map :=
+    @map_agree_auth _ _ _ _ _ pstore_G_map_G γ map.
+  #[local] Definition pstore_map_elem γ n l σ :=
+    @map_agree_elem _ _ _ _ _ pstore_G_map_G γ n (l,σ).
+
+  Lemma extract_unaliased g :
+    ([∗ set] '(r, (l, v), r') ∈ g, r ↦ ’Diff{ #(LiteralLoc l), v, #(LiteralLoc r') }) -∗
+    ⌜unaliased g⌝.
+  Proof.
+    iIntros "Hg" (???????).
+    destruct_decide (decide (a0 = a2 ∧ a1 = a3)). done.
+    rewrite (big_sepS_delete _ _ (a, a0, a1)). set_solver.
+    rewrite (big_sepS_delete _ _ (a, a2, a3)). set_solver.
+    iDestruct "Hg" as "(?&?&_)". destruct a0,a2.
+    iDestruct (mapsto_ne with "[$][$]") as "%". congruence.
+  Qed.
+
+  (* NB our invariant asserts that g is indeed a rooted tree: a rooted DAG
+     with unicity of paths. Indeed, from the set of pointsto we can extract [unaliased],
+     (see [extract_unaliased]), and a DAG with unaliased guarantees unicity of paths
+     (see [acyclic_unaliased_impl_uniq_path] ) *)
+
+  #[local] Definition pstore (γ:gname) (t:val) (σ:gmap loc val) : iProp Σ :=
+    ∃ (t0 r:loc)
+      (σ0:gmap loc val) (* the global map, with all the points-to ever allocated *)
+      (g:graph_store) (* the global graph *)
+      (M:map_model) (* the map model, associating to each node its model *)
+      (C:gmap nat (loc * gmap loc val)), (* the model of snapshots *)
+    ⌜t=#t0 /\ store_inv M g r σ σ0 /\ coherent M σ0 g /\ rooted_dag g r /\ snap_inv M C⌝ ∗
+    t0 ↦ #(LiteralLoc r) ∗
+    r ↦ §Root ∗
+    pstore_map_auth γ C ∗
+    ([∗ map] l ↦ v ∈ σ0, l ↦ v) ∗
+    ([∗ set] x ∈ g, let '(r,(l,v),r') := x in r ↦ ’Diff{ #(LiteralLoc l), v, #(LiteralLoc r') }) .
+
+  Definition open_inv : string :=
+    "[%t0 [%r [%σ0 [%g [%M [%C ((->&%Hinv&%Hcoh&%Hgraph&%Hsnap)&Ht0&Hr&HC&Hσ0&Hg)]]]]]]".
+
+  Definition pstore_snapshot γ t s σ : iProp Σ :=
+    ∃ l n, ⌜s=ValTuple [t;#l]⌝ ∗ pstore_map_elem γ n l σ.
+
+  #[global] Instance pstore_snapshot_timeless γ t s σ :
+    Timeless (pstore_snapshot γ t s σ).
+  Proof. apply _. Qed.
+  #[global] Instance pstore_snapshot_persistent γ t s σ :
+    Persistent (pstore_snapshot γ t s σ).
+  Proof. apply _. Qed.
+
+  Lemma pstore_create_spec :
+    {{{ True }}}
+      pstore_create ()
+    {{{ t γ,
+      RET t;
+        pstore γ t ∅
+    }}}.
+  Proof.
+    iIntros "%Φ _ HΦ".
+    wp_rec.
+    wp_alloc r as "Hroot".
+    wp_alloc t0 as "Ht0".
+    iMod (map_agree_alloc ∅) as "[%γ ?]".
+    iApply "HΦ". iModIntro.
+    iExists t0,r,∅,∅,{[r := ∅]},∅. iFrame.
+    rewrite !big_sepM_empty big_sepS_empty !right_id.
+    iPureIntro. split_and!; first done.
+    { constructor.
+      { rewrite dom_singleton_L vertices_empty //. set_solver. }
+      { set_solver. }
+      { rewrite lookup_insert //. }
+      { intros ????? Hr.
+        rewrite !lookup_singleton_Some.
+        inversion Hr; set_solver. } }
+    { constructor.
+      { intros ??. rewrite lookup_singleton_Some. intros (->&->). reflexivity. }
+      { intros ????. set_solver. } }
+    { eauto using rooted_dag_empty. }
+    { intros ??. set_solver. }
+  Qed.
+
+  Lemma use_locs_of_edges_in g r xs r' X :
+    locs_of_edges_in g X ->
+    path g r xs r' ->
+    (list_to_set (proj2 <$> xs).*1) ⊆ X.
+  Proof.
+    intros He.
+    induction 1. set_solver.
+    apply He in H. set_solver.
+  Qed.
+
   Lemma pstore_ref_spec γ t σ v :
     {{{
       pstore γ t σ
@@ -630,7 +761,7 @@ Section pstore_G.
       pstore_ref v
     {{{ l,
       RET #l;
-      ⌜σ !! l = None⌝ ∗
+      ⌜l ∉ dom σ⌝ ∗
       pstore γ t (<[l := v]> σ)
     }}}.
   Proof.
@@ -644,65 +775,45 @@ Section pstore_G.
       apply elem_of_dom in Hl. destruct Hl.
       iDestruct (big_sepM_lookup with "Hσ0") as "Hl_"; first done.
       iDestruct (mapsto_ne with "Hl Hl_") as %?. done. }
-    assert (σr !! l = None) as Hl.
-    { eapply not_elem_of_dom. apply not_elem_of_dom in Hl0.
-      intros ?. apply Hl0. destruct Hcoh. eapply incl_dom_incl; eauto. }
     assert (σ !! l = None).
-    { eapply not_elem_of_dom. intros ?. apply not_elem_of_dom in Hl. apply Hl.
-      destruct Hinv.
-      eapply incl_dom_incl. 2:done. done. }
+    { eapply not_elem_of_dom. apply not_elem_of_dom in Hl0.  destruct Hinv as [_ X].
+      apply incl_dom_incl in X. set_solver. }
     iDestruct (mapsto_ne with "Hl Hr") as %Hlr.
 
-    iAssert ⌜forall x y, (r,x,y) ∉ g⌝%I as "%Hrg".
-    { iIntros (???). destruct a. iDestruct (big_sepS_elem_of with "Hg") as "?". done.
-      iClear "Ht0 Hl".
-      iDestruct (mapsto_ne with "[$][$]") as "%". congruence. }
-
-
-    iModIntro. iStep.
-    iExists t0,r, (<[l:=v]>σ0),(<[l := v]> σr),g,(<[r:=<[l:=v]>σr]>M),C.
+    iModIntro. iSplitR. iPureIntro. by eapply not_elem_of_dom.
+    iExists t0,r, (<[l:=v]>σ0),g,((fun σ => <[l:=v]>σ)<$> M),C.
 
     rewrite big_sepM_insert //. iFrame.
     iPureIntro. split_and !; eauto.
     { destruct Hinv as [X1 X2 X3 X4].
       constructor.
-      { rewrite dom_insert_L; set_solver. }
+      { rewrite dom_fmap_L; set_solver. }
       { eauto using gmap_included_insert. }
-      { rewrite lookup_insert //. }
-      { intros r1 ds r2 σ1 σ2 Hr. generalize Hr. intros Hreach.
-        destruct_decide (decide (r1=r)).
-        { subst. rewrite lookup_insert. inversion 1. subst.
-          inversion Hr; subst.
-          2:{ exfalso. set_solver. }
-          rewrite lookup_insert. inversion 1. done. }
-        { rewrite lookup_insert_ne //. intros Hr1.
-          destruct_decide (decide (r2=r)).
-          { subst. rewrite lookup_insert. inversion 1. subst.
-            eapply X4 in Hr. 2,3:done.
-            destruct Hcoh as [Z1 Z2].
-            eapply use_locs_of_edges_in in Z2. 2:done.
-            rewrite apply_diffl_insert_ne.
-            { apply not_elem_of_dom in Hl0. set_solver. }
-            apply gmap_included_insert_notin; last done.
-            apply incl_dom_incl in Z1. apply incl_dom_incl in Hr.
-            rewrite dom_apply_diffl in Hr.
-            apply not_elem_of_dom in Hl0,Hl. set_solver. }
-          { rewrite lookup_insert_ne //. eauto. } } } }
+      { rewrite lookup_fmap X3 //. }
+      { intros r1 ds r2 σ1 σ2 Hr. rewrite !lookup_fmap. generalize Hr. intros Hreach.
+        intros Hr1 Hr2.
+        destruct (M !! r1) eqn:Hor1. 2:simpl in *; congruence.
+        inversion Hr1. subst.
+        destruct (M !! r2) eqn:Hor2. 2:simpl in *; congruence.
+        inversion Hr2. subst.
+        destruct Hcoh as [Z1 Z2].
+        eapply use_locs_of_edges_in in Z2. 2:done.
+        rewrite apply_diffl_insert_ne.
+        { apply not_elem_of_dom in Hl0. set_solver. }
+        { f_equal. eauto. } } }
     { destruct Hcoh as [X1 X2].
       constructor.
-      { eauto using gmap_included_insert. }
+      { intros r' ?. rewrite lookup_fmap. intros E.
+        destruct (M !! r') eqn:Hor. 2:simpl in *; congruence.
+        inversion E. subst. rewrite !dom_insert_L. set_solver. }
       { intros. rewrite dom_insert_L. intros ??. set_solver. } }
-    { intros ? r' ? HC. apply Hsnap in HC. destruct HC as (?&?&?).
-      destruct_decide (decide (r'=r)).
-      { subst. eexists. rewrite lookup_insert. split; first done.
-        destruct Hinv as [X1 X2 X3 X4].
-        rewrite X3 in H0. inversion H0. subst.
-        apply gmap_included_insert_notin; last done.
-        apply incl_dom_incl in H1. intros X. apply H1 in X.
-        apply not_elem_of_dom in Hl. done. }
-      { eexists. rewrite lookup_insert_ne //. } }
+    { intros ? r' ? HC. apply Hsnap in HC. destruct HC as (x&Hx&?).
+      exists (<[l:=v]>x). rewrite lookup_fmap Hx. split. done.
+      apply gmap_included_insert_notin; last done.
+      apply incl_dom_incl in H0. intros X. apply H0 in X.
+      destruct Hcoh as [X1 X2]. apply X1 in Hx.
+      apply not_elem_of_dom in Hl0. set_solver. }
   Qed.
-
 
   Lemma pstore_get_spec {γ t σ l} v :
     σ !! l = Some v →
@@ -719,10 +830,8 @@ Section pstore_G.
     wp_rec. iStep 4. iModIntro.
 
     iDestruct (big_sepM_lookup_acc _ _ l v with "[$]") as "(?&Hσ0)".
-    { destruct Hcoh as [X1 X2].
-      destruct Hinv as [Z1 Z2 Z3].
-      assert (σ ⊆ σ0) as T. etrans; eauto.
-      specialize (T l). rewrite Hl in T. destruct (σ0!!l); naive_solver. }
+    { destruct Hinv as [_ Hincl _ _].
+      specialize (Hincl l). rewrite Hl in Hincl. destruct (σ0!!l); naive_solver. }
 
     iSteps.
   Qed.
@@ -742,9 +851,10 @@ Section pstore_G.
     wp_rec. iStep 8. iModIntro.
     wp_alloc r' as "Hr'".
 
-    assert (l ∈ dom σ0) as Hl0.
-    { destruct Hcoh as [Z1 _]. destruct Hinv as [_ Z2]. apply incl_dom_incl in Z1,Z2. eauto. }
-    apply elem_of_dom in Hl0. destruct Hl0 as (w&Hl0).
+    assert (exists w, σ0 !! l = Some w) as (w&Hl0).
+    { apply elem_of_dom. destruct Hinv as [_ Hincl].
+      apply incl_dom_incl in Hincl.
+      set_solver. }
 
     iDestruct (big_sepM_insert_acc with "Hσ0") as "(?&Hσ0)". done.
     wp_load. wp_load. wp_store. iStep 4. iModIntro.
@@ -756,69 +866,53 @@ Section pstore_G.
     { iClear "Ht0". iDestruct (mapsto_ne with "[$][$]") as %?. done. }
 
     iAssert ⌜r' ∉ vertices g⌝%I as %Hr'.
-    { iClear "Ht0". iIntros (Hr'). destruct Hgraph as [X1 X2].
+    { iIntros (Hr'). destruct Hgraph as [X1 X2].
       apply X1 in Hr'. destruct Hr' as (?&Hr'). inversion Hr'; subst.
       { done. }
       { destruct b. iDestruct (big_sepS_elem_of with "[$]") as "?". done.
-        iDestruct (mapsto_ne with "[$][$]") as %?. congruence. } }
+        iDestruct (mapsto_ne r' r' with "[$][$]") as %?. congruence. } }
 
-    iAssert ⌜forall x y, (r,x,y) ∉ g⌝%I as "%Hrg".
-    { iIntros (???). destruct a. iDestruct (big_sepS_elem_of with "Hg") as "?". done.
-      iClear "Ht0 Hr'".
-      iDestruct (mapsto_ne with "[$][$]") as "%". congruence. }
-
-    iModIntro. iExists t0,r',(<[l:=v]> σ0),(<[l:=v]> σr),({[(r,(l,w),r')]} ∪ g), (<[r':=<[l:=v]> σr]>M),C.
+    iModIntro. iExists t0,r',(<[l:=v]> σ0),({[(r,(l,w),r')]} ∪ g), (<[r':=<[l:=v]> σ0]>M),C.
     rewrite big_sepS_union.
     { apply disjoint_singleton_l. intros ?. apply Hr'.
       apply elem_of_vertices. eauto. }
-    rewrite big_sepS_singleton. iFrame.
-    iPureIntro.
-    { split_and!; first done.
-      { destruct Hinv as [X1 X2 X3 X4].
-        constructor.
-        { rewrite dom_insert_L vertices_union vertices_singleton //. set_solver. }
-        { apply gmap_included_insert. done. }
-        { rewrite lookup_insert //. }
-        { intros r1 ds r2 σ1 σ2 Hreach.
-          destruct_decide (decide (r'=r1)).
-          { subst. rewrite lookup_insert. inversion_clear 1.
-            inversion Hreach. subst.
-            2:{ exfalso. subst. rewrite /edge elem_of_union in H0.
-                destruct H0. set_solver. apply Hr'. apply elem_of_vertices. set_solver. }
-            rewrite lookup_insert. inversion 1. done. }
-          rewrite lookup_insert_ne //. intros E1.
-          destruct_decide (decide (r2=r')).
-          { subst. rewrite lookup_insert. inversion 1. subst.
-            apply reachable_add_end in Hreach. 2,3:eauto.
-            destruct Hreach as [(->&->)|(ds'&->&Hreach)].
-            { congruence. }
-            specialize (X4 _ _ _ _ _ Hreach E1 X3). etrans. apply X4.
-            rewrite apply_diffl_app. simpl. rewrite insert_insert.
-            destruct Hcoh as [Z1 _ ]. rewrite insert_id //.
-            assert (exists z, σr !! l = Some z) as (?&Hz).
-            { apply elem_of_dom. eapply incl_dom_incl. done. done. }
-            specialize (Z1 l). rewrite Hl0 Hz in Z1. naive_solver. }
-          { rewrite lookup_insert_ne //. intros. eapply X4; eauto.
-            apply reachable_cycle_end_inv_aux in Hreach; eauto. } } }
-      { destruct Hcoh as [X1 X2].
-        constructor.
-        { eauto using gmap_included_insert. }
-        { intros ?. set_solver. } }
-      { eauto using rooted_dag_add. }
-      { intros ? r0 ? HC. apply Hsnap in HC. destruct HC as (?&HC&?).
-        destruct_decide (decide (r0=r')).
-        { exfalso. subst. destruct Hinv as [X1 X2 X3].
-          assert (r' ∉ dom M) as F by set_solver. apply F. by eapply elem_of_dom. }
-        rewrite lookup_insert_ne //. eauto. } }
-  Qed.
-
-  Definition pstore_snapshot γ t s σ : iProp Σ :=
-    ∃ l n, ⌜s=ValTuple [t;#l]⌝ ∗ pstore_map_elem γ n l σ.
-
-  #[global] Instance pstore_snapshot_persistent γ t s σ :
-    Persistent (pstore_snapshot γ t s σ).
-  Proof.
-    apply _.
+    rewrite big_sepS_singleton. iFrame. iPureIntro.
+    split_and!; first done.
+    { destruct Hinv as [X1 X2 X3 X4].
+      constructor.
+      { rewrite dom_insert_L vertices_union vertices_singleton //. set_solver. }
+      { apply gmap_included_insert. done. }
+      { rewrite lookup_insert //. }
+      { intros r1 ds r2 σ1 σ2 Hreach.
+        destruct_decide (decide (r'=r1)).
+        { subst. rewrite lookup_insert. inversion_clear 1.
+          inversion Hreach. subst.
+          2:{ exfalso. subst. rewrite /edge elem_of_union in H0.
+              destruct H0. set_solver. apply Hr'. apply elem_of_vertices. set_solver. }
+          rewrite lookup_insert. inversion 1. done. }
+        rewrite lookup_insert_ne //. intros E1.
+        destruct_decide (decide (r2=r')).
+        { subst. rewrite lookup_insert. inversion 1. subst.
+          apply path_add_inv_r in Hreach; try done.
+          destruct Hreach as [(->&->)|(ds'&->&Hreach)].
+          { congruence. }
+          specialize (X4 _ _ _ _ _ Hreach E1 X3).
+          rewrite fmap_app apply_diffl_snoc insert_insert insert_id //. }
+        { rewrite lookup_insert_ne //. intros. eapply X4; eauto.
+          apply path_cycle_end_inv_aux in Hreach; eauto. } } }
+    { destruct Hcoh as [X1 X2].
+      constructor.
+      { intros r0 ?. destruct_decide (decide (r0=r')).
+        { subst. rewrite lookup_insert. inversion 1. done. }
+        rewrite lookup_insert_ne //. intros HM.
+        apply X1 in HM. rewrite dom_insert_lookup_L //. }
+      { intros ?. set_solver. } }
+    { eauto using rooted_dag_add. }
+    { intros ? r0 ? HC. apply Hsnap in HC. destruct HC as (?&HC&?).
+      destruct_decide (decide (r0=r')).
+      { exfalso. subst. destruct Hinv as [X1 X2 X3].
+        assert (r' ∉ dom M) as F by set_solver. apply F. by eapply elem_of_dom. }
+      rewrite lookup_insert_ne //. eauto. }
   Qed.
 
   Lemma pstore_capture_spec γ t σ :
@@ -839,16 +933,13 @@ Section pstore_G.
     { apply not_elem_of_dom. apply is_fresh. }
     iModIntro.
     iSplitR "Hsnap". 2:iSteps.
-    iExists _,_,_,_,_,_,_. iFrame.
+    iExists _,_,_,_,_,_. iFrame.
     iPureIntro. split_and!; eauto.
     intros ? r' ? HC.
     destruct_decide (decide (n=fresh (dom C))).
-    { subst. rewrite lookup_insert in HC. inversion HC. subst r' σ1.
-      destruct Hinv as [X1 X2 X3 X4].
-      assert (exists σ', M!! r = Some σ') as (σ',HM).
-      { apply elem_of_dom. set_solver. }
-      exists σ'. split; first done. naive_solver. }
-    { rewrite lookup_insert_ne // in HC. eauto using Hsnap. }
+    { subst. rewrite lookup_insert in HC. inversion HC. subst.
+      destruct Hinv. eauto. }
+    { rewrite lookup_insert_ne // in HC. eauto. }
   Qed.
 
   Definition fsts  (ys:list (loc*(loc*val)*loc)) : list val :=
@@ -856,7 +947,8 @@ Section pstore_G.
 
   Lemma pstore_collect_spec_aux (r r':loc) t' (xs:list val) (ys:list (loc*(loc*val)*loc)) (g:graph_store) :
     path g r ys r' ->
-    {{{ r' ↦ §Root ∗
+    {{{
+        r' ↦ §Root ∗
         lst_model t' xs ∗
         ([∗ set] '(r, (l, v), r') ∈ g, r ↦ ’Diff{ #(LiteralLoc l), v, #(LiteralLoc r') })
     }}}
@@ -886,8 +978,9 @@ Section pstore_G.
 
  Lemma pstore_collect_spec (r r':loc) (ys:list (loc*(loc*val)*loc)) (g:graph_store) :
    path g r ys r' ->
-   {{{ r' ↦ §Root ∗
-        ([∗ set] '(r, (l, v), r') ∈ g, r ↦ ’Diff{ #(LiteralLoc l), v, #(LiteralLoc r') })
+   {{{
+      r' ↦ §Root ∗
+      ([∗ set] '(r, (l, v), r') ∈ g, r ↦ ’Diff{ #(LiteralLoc l), v, #(LiteralLoc r') })
    }}}
      pstore_collect #r §Nil
    {{{ t,
@@ -902,45 +995,6 @@ Section pstore_G.
     iDestruct (pstore_collect_spec_aux with "[$]") as "Go". done.
     iApply "Go". rewrite -rev_alt //. Unshelve. apply _.
   Qed.
-
-  Lemma apply_diffl_snoc_notin x xs σ :
-    x.1 ∉ xs.*1 ->
-    apply_diffl (xs ++ [x]) σ = apply_diffl (x::xs) σ.
-  Proof.
-    revert σ. induction xs; intros σ.
-    { done. }
-    rewrite -app_comm_cons =>?. destruct a. simpl.
-    rewrite IHxs. set_solver. destruct x. simpl.
-    rewrite insert_commute //. set_solver.
-  Qed.
-
-  Lemma apply_diffl_snoc xs l v σ :
-    apply_diffl (xs ++ [(l,v)]) σ = apply_diffl xs (<[l:=v]> σ).
-  Proof.
-    revert σ. induction xs. done.
-    intros σ. rewrite -app_comm_cons. simpl.
-    rewrite IHxs //.
-  Qed.
-
-  Record revset (xs ys: list (loc*(loc*val)*loc)) σ :=
-    { re1 :  forall r l r' v,
-        (r,(l,v),r') ∈ xs -> (exists v', σ !! l = Some v' /\ (r',(l,v'),r) ∈ ys);
-      re2 : forall r l r' v',
-        σ !! l = Some v' ->
-        (r',(l,v'),r) ∈ ys ->
-        exists v, (r,(l,v),r') ∈ xs }.
-
-  (* undo applied generated orig_store *)
-  Inductive undo :
-    list (loc*(loc*val)*loc) -> list (loc*(loc*val)*loc) -> gmap loc val -> Prop :=
-  | undo_nil :
-    forall σ, undo [] [] σ
-  | undo_cons :
-    forall σ r l v v' r' xs ys,
-      σ !! l = Some v' ->
-      undo xs ys (<[l:=v]> σ) ->
-      undo (xs++[(r,(l,v),r')]) ((r',(l,v'),r)::ys) σ
-  .
 
   Lemma use_path r g (xs:list (loc*(loc*val)*loc)) r0 x r1 r':
     list_to_set xs ⊆ g ->
@@ -962,13 +1016,33 @@ Section pstore_G.
       eapply path_weak. done. set_solver. }
   Qed.
 
-  Lemma acyclic_weak `{Countable A} `{Countable B} (g1 g2:graph A B) :
-    acyclic g1 ->
-    g2 ⊆ g1 ->
-    acyclic g2.
+  (* [undo xs ys σ] asserts [mirror xs ys] and that [σ = apply_diffl (proj2 <$> ys ++ xs) σ],
+     ie, ys undo the changes of xs *)
+  Inductive undo :
+    list (loc*(loc*val)*loc) -> list (loc*(loc*val)*loc) -> gmap loc val -> Prop :=
+  | undo_nil :
+    forall σ, undo [] [] σ
+  | undo_cons :
+    forall σ r l v v' r' xs ys,
+      σ !! l = Some v' ->
+      undo xs ys (<[l:=v]> σ) ->
+      undo (xs++[(r,(l,v),r')]) ((r',(l,v'),r)::ys) σ.
+
+  Lemma use_undo xs ys σ :
+    undo xs ys σ ->
+    σ = apply_diffl (proj2 <$> ys ++ xs) σ.
   Proof.
-    intros Hacy ? ???. eapply Hacy. by eapply path_weak.
+    induction 1.
+    { done. }
+    rewrite !assoc_L fmap_app apply_diffl_snoc.
+    rewrite -app_comm_cons fmap_cons apply_diffl_cons.
+    rewrite -IHundo insert_insert insert_id //.
   Qed.
+
+  Lemma undo_mirror xs ys g :
+    undo xs ys g ->
+    mirror xs ys.
+  Proof. induction 1; eauto using mirror_cons,mirror_nil. Qed.
 
   Lemma pstore_revert_spec_aux g g1 r t g2 xs r' w σ σ0 :
     locs_of_edges_in g2 (dom σ) ->
@@ -994,7 +1068,7 @@ Section pstore_G.
       iStep 4. iModIntro.
       iApply (wp_lst_match_Nil with "[$]") .
       inversion Hpath. subst. wp_store. iModIntro.
-      iApply "HΦ". iExists nil. rewrite right_id_L. iFrame.
+      iApply "HΦ". iExists nil. rewrite !right_id_L. iFrame.
       iPureIntro. eauto using undo_nil. }
     { wp_rec. simpl. rewrite rev_unit. simpl.
       iStep 4. iModIntro.
@@ -1104,62 +1178,24 @@ Section pstore_G.
     intros Z ? a b c d ?. eapply (Z a b c d). set_solver.
   Qed.
 
-
-  Lemma apply_diffl_included xs σ1 σ2 :
-    σ1 ⊆ σ2 ->
-    apply_diffl xs σ1 ⊆ apply_diffl xs σ2.
-  Proof.
-    revert σ1 σ2. induction xs as [|(?,?)]; intros;
-      [ done | eauto using gmap_included_insert ].
-  Qed.
-
-  Lemma undo_same_fst_label xs ys σ r l v r' :
+  Lemma undo_same_fst_label xs ys r l v r' σ :
     undo xs ys σ ->
     (r, (l, v), r') ∈ (list_to_set ys :  gset (loc*(loc*val)*loc)) ->
     l ∈ (list_to_set (proj2 <$> xs).*1 : gset loc).
   Proof.
     revert xs σ. induction ys as [|(?,?)]. set_solver.
     intros xs σ. inversion 1. subst.
-    simpl. rewrite !fmap_app list_to_set_app_L.
+    simpl. rewrite !fmap_app list_to_set_app_L. simpl in *. subst.
     destruct_decide (decide ((r, (l, v), r') = (r'0, (l1, v'), l0))) as Heq.
     { inversion Heq. subst. intros _. set_solver. }
     intros ?. simpl. apply elem_of_union. left. eapply IHys. done. set_solver.
-  Qed.
-
-  Lemma path_restrict  `{Countable A} `{Countable B} (g:graph A B) r xs r' :
-    path g r xs r' ->
-    path (list_to_set xs) r xs r'.
-  Proof.
-    induction 1.
-    { apply path_nil. }
-    { apply path_cons. set_solver.
-      eapply path_weak. done. set_solver. }
-  Qed.
-
-  Lemma path_all_in `{Countable A} `{Countable B} (g:graph A B) a1 xs a2 :
-    path g a1 xs a2 ->
-    list_to_set xs ⊆ g.
-  Proof.
-    induction 1; simpl; set_solver.
-  Qed.
-
-  Lemma path_inv_r (g:gset (loc*(loc*val)*loc)) x bs z :
-    path g x bs z ->
-    (x = z /\ bs = nil) ∨ ∃ bs' b y, bs = bs' ++ [(y,b,z)] /\ path g x bs' y ∧ (y,b,z) ∈ g.
-  Proof.
-    induction 1.
-    { naive_solver.  }
-    right. destruct IHpath as [(->&->)|(bs'&b'&y&->&?&?)].
-    { exists nil. eexists _,_. split; first done. split. eauto using path_nil. naive_solver. }
-    { exists ((a1, b, a2) :: bs'). eexists _,_. rewrite app_comm_cons //. split_and !; try done.
-      apply path_cons; eauto. }
   Qed.
 
   Definition diff_last {A:Type} (ys1 ys2:list A) :=
     match last ys1,last ys2 with Some x,Some y => x ≠ y | _,_ => True end.
 
   Lemma path_extract_suffix (g:gset (loc*(loc*val)*loc)) a1 a2 xs1 r xs2 :
-    kindofinj g ->
+    unaliased g ->
     path g a1 xs1 r ->
     path g a2 xs2 r  ->
     exists ys1 ys2 xs,
@@ -1189,29 +1225,12 @@ Section pstore_G.
     eexists _,_,(xs++[(y, b, r)]). rewrite !assoc_L. done.
   Qed.
 
-  Lemma elem_of_middle {A:Type} (x:A) (xs:list A) :
-    x ∈ xs ->
-    exists (l1 l2:list A), xs = l1 ++ x::l2.
-  Proof.
-    intros Hx. apply elem_of_list_lookup_1 in Hx.
-    destruct Hx as (?&?).
-    eexists _,_. symmetry. eapply take_drop_middle. done.
-  Qed.
-
   Lemma diff_last_app_middle {A:Type} x (l1' l2' l1 l2:list A) :
     diff_last (l1' ++ x :: l2') (l1 ++ x :: l2) ->
     diff_last (x :: l2') (x :: l2).
   Proof.
     unfold diff_last. rewrite !last_app !last_cons.
     destruct (last l2),(last l2'); eauto.
-  Qed.
-
-  Lemma list_case_r {A:Type} (l:list A) :
-    l = nil \/ exists (l':list A) x, l = l' ++ [x].
-  Proof.
-    induction l using rev_ind.
-    naive_solver. right.
-    destruct IHl as [-> | (?&?&->)]; eauto.
   Qed.
 
   Lemma diff_last_irrefl {A:Type} (l:list A) :
@@ -1225,7 +1244,7 @@ Section pstore_G.
 
   Lemma path_use_diff_last (g:gset (loc*(loc*val)*loc)) a1 a2 ys1 ys2 xs r :
     acyclic g ->
-    kindofinj g ->
+    unaliased g ->
     path g a1 (ys1 ++ xs) r ->
     path g a2 (ys2 ++ xs) r  ->
     diff_last ys1 ys2 ->
@@ -1247,7 +1266,8 @@ Section pstore_G.
       assert (x2=proj1 x).
       { inversion Hp2. subst. done. }
       subst.
-      eapply use_kindofinj in Hp1; eauto.
+      eapply acyclic_unaliased_impl_uniq_path in Hp2; eauto.
+      apply Hp2 in Hp1.
       rewrite !app_comm_cons in Hp1.
       apply app_inv_tail in Hp1.
       apply diff_last_app_middle in Hdiff.
@@ -1269,49 +1289,6 @@ Section pstore_G.
       { inversion Hp2'. subst. done. }
       rewrite -app_comm_cons in Hp2.
       eapply Hacy in Hp2. congruence. }
-  Qed.
-
-  Lemma path_middle (g:graph loc (loc*val)) x xs ys z :
-    path g x (xs ++ ys) z ->
-    exists y, path g x xs y /\ path g y ys z.
-  Proof.
-    revert g x ys z. induction xs; intros g x ys z.
-    { simpl. eauto using path_nil. }
-    inversion 1; simpl in *; subst.
-    apply IHxs in H5. destruct H5 as (y,(?&?)).
-    exists y. split; last done. eauto using path_cons.
-  Qed.
-
-  Definition undo_weak (xs ys:list (loc*(loc*val)*loc)) :=
-    forall r x r', (r,x,r') ∈ xs -> exists x', (r',x',r) ∈ ys.
-
-  Lemma path_app (g:graph loc (loc*val)) x3 x1 xs ys x2 :
-    path g x1 xs x3 ->
-    path g x3 ys x2 ->
-    path g x1 (xs++ys) x2.
-  Proof.
-    intros Hp.
-    revert x2 ys. induction Hp. eauto.
-    intros. rewrite -app_comm_cons. apply path_cons. set_solver.
-    eauto.
-  Qed.
-
-  Lemma use_undo ys2 us ys g r y :
-    undo_weak (ys2 ++ us) ys ->
-    path g r ys2 y ->
-    exists zs, path (list_to_set ys) y zs r.
-  Proof.
-    intros Hundo Hpath.
-    revert us ys Hundo. induction Hpath; intros us' ys Hundo.
-    { exists nil. apply path_nil. }
-    assert (exists b', (a2,b',a1) ∈ ys) as (b'&Hb').
-    { eapply (Hundo _ b). set_solver. }
-    assert (undo_weak (bs ++ us') ys) as Hundo'.
-    { intros ????. eapply (Hundo _ x). set_solver. }
-    apply IHHpath in Hundo'.
-    destruct Hundo' as (π&?).
-    exists (π ++ [(a2, b', a1)]). eapply path_app; first done.
-    apply path_cons. 2:apply path_nil. set_solver.
   Qed.
 
   Lemma diff_last_comm {A:Type} (l1 l2:list A) :
@@ -1342,94 +1319,11 @@ Section pstore_G.
       set_solver. apply path_cons. set_solver. done. }
   Qed.
 
-  Lemma use_undo_weak' xs ys g r y :
-    undo_weak xs ys ->
-    path g r xs y ->
-    exists zs, path (list_to_set ys) y zs r /\ length xs = length zs.
-  Proof.
-    intros Hweak.
-    induction 1.
-    { exists nil. split. apply path_nil. done. }
-    { destruct IHpath as (zs&Hzs&?).
-      { intros ????. eapply Hweak. apply elem_of_cons. eauto. }
-      destruct (Hweak a1 b a2) as (b'&Hb'). set_solver.
-      exists (zs ++ [(a2, b', a1)]). split.
-      { eapply path_app. done.
-        apply path_cons. set_solver. apply path_nil. }
-      { rewrite app_length. simpl. lia. } }
-  Qed.
-
-  Inductive undo0 :
-    list (loc*(loc*val)*loc) -> list (loc*(loc*val)*loc) -> Prop :=
-  | undo0_nil :
-    undo0 [] []
-  | undo0_cons :
-    forall r x x' r' xs ys,
-      undo0 xs ys  ->
-      undo0 (xs++[(r,x,r')]) ((r',x',r)::ys).
-
-  Lemma undo_undo0 xs ys σ :
-    undo xs ys σ ->
-    undo0 xs ys.
-  Proof.
-    induction 1; eauto using undo0_nil, undo0_cons.
-  Qed.
-
-  Lemma undo0_snoc ys xs a a' x x' :
-    undo0 ys xs ->
-    undo0 ((a,x,a') :: ys) (xs ++ [(a',x',a)]).
-  Proof.
-    induction 1.
-    { apply (undo0_cons _ _ _ _ nil nil). apply undo0_nil. }
-    rewrite -!app_comm_cons app_comm_cons. by apply undo0_cons.
-  Qed.
-
-  Lemma undo0_symm xs ys :
-    undo0 xs ys -> undo0 ys xs.
-  Proof.
-    induction 1. eauto using undo0_nil.
-    apply undo0_snoc. eauto.
-  Qed.
-
-  Lemma undo0_undo_weak xs ys :
-    undo0 xs ys ->
-    undo_weak xs ys.
-  Proof.
-    induction 1. intros ?. set_solver.
-    intros ???. rewrite elem_of_app elem_of_list_singleton.
-    intros [X|X].
-    { apply IHundo0 in X. set_solver. }
-    { set_solver. }
-  Qed.
-
-  Definition pathlike (ys:list (loc*(loc*val)*loc)) r :=
-    forall a b a', (a,b,a') ∈ ys -> a' = r \/ exists b' a'', (a',b',a'') ∈ ys.
-
-  Lemma use_undo' g r xs ys y :
-    path g r xs y ->
-    undo0 xs ys ->
-    pathlike ys r.
-  Proof.
-    intros Hpath Hundo. generalize Hundo. intros Hundo'.
-    apply undo0_symm in Hundo.
-    apply undo0_undo_weak in Hundo.
-    intros ??? Hys. apply Hundo in Hys. destruct Hys as (?&?).
-    apply elem_of_middle in H. destruct H as (l1&l2&->).
-    apply path_app_inv in Hpath. destruct Hpath as (r'&E1&E2).
-    assert (r'=a') as ->.
-    { inversion E2. subst. done. }
-    apply path_inv_r in E1.
-    destruct E1 as [|(?&?&?&->&Hpath&?)].
-    naive_solver.
-    apply undo0_undo_weak in Hundo'.
-    destruct (Hundo' x2 x1 a'). set_solver. set_solver.
-  Qed.
-
   Lemma path_cannot_escape (x:(loc * diff * loc)) (xs ys:list (loc * diff * loc)) (g1: graph loc (loc*val)) a a' r :
     (forall x l', ¬ (r,x,l') ∈ (g1 ∪ list_to_set ys)) ->
-    kindofinj (g1 ∪ list_to_set ys) ->
+    unaliased (g1 ∪ list_to_set ys) ->
     x ∈ (list_to_set ys : gset _) ->
-    (forall a b a', (a,b,a') ∈ ys -> a' = r \/ exists b' a'', (a',b',a'') ∈ ys) ->
+    pathlike ys r ->
     path (g1 ∪ list_to_set ys) a (x :: xs) a' ->
     path (list_to_set ys) a (x::xs) a'.
   Proof.
@@ -1448,8 +1342,8 @@ Section pstore_G.
 
   Lemma path_in_seg_complete (r a a':loc) (x:(loc * diff * loc)) (xs0 xs1 ys: list (loc * diff * loc)) (g1:graph loc (loc*val)) :
     (forall x l', ¬ (r,x,l') ∈ (g1 ∪ list_to_set ys)) -> (* root has no succ *)
-    kindofinj (g1 ∪ list_to_set ys) ->
-    (forall a b a', (a,b,a') ∈ ys -> a' = r \/ exists b' a'', (a',b',a'') ∈ ys) -> (* ys is "closed "*)
+    unaliased (g1 ∪ list_to_set ys) ->
+    pathlike ys r ->
     path (g1 ∪ list_to_set ys) a xs0 a' ->
     path (list_to_set ys) a' (x :: xs1) a ->
     exists zs, path (list_to_set ys) a zs a'.
@@ -1468,28 +1362,19 @@ Section pstore_G.
     destruct (Hinj _ _ _ _ _ H Z). set_solver.
   Qed.
 
-  Lemma undo0_vertices xs ys :
-    undo0 xs ys ->
-    vertices (list_to_set ys) = vertices (list_to_set xs).
-  Proof.
-    revert xs. induction ys; intros xs; inversion 1; subst. done.
-    simpl. rewrite list_to_set_app_L !vertices_union !vertices_singleton. simpl.
-    erewrite IHys; last done. rewrite vertices_empty. set_solver.
-  Qed.
-
-  Lemma undo_preserves_rooted_dag g xs ys rs r :
+  Lemma undo_preserves_rooted_dag (g:graph loc (loc*val)) xs ys rs r :
     (forall x l', ¬ (rs,x,l') ∈ (list_to_set ys ∪ g ∖ list_to_set xs)) -> (* root has no succ *)
-    kindofinj g ->
-    kindofinj (list_to_set ys ∪ g ∖ list_to_set xs) ->
+    unaliased g ->
+    unaliased (list_to_set ys ∪ g ∖ list_to_set xs) ->
     path g rs xs r ->
-    undo0 xs ys ->
+    mirror xs ys ->
     rooted_dag g r ->
     rooted_dag (list_to_set ys ∪ g ∖ list_to_set xs) rs.
   Proof.
-    intros Hnr Hinj Hinj' Hpath Hundo Hroot. inversion Hroot as [X1 X2].
+    intros Hnr Hinj Hinj' Hpath Hmirror Hroot. inversion Hroot as [X1 X2].
     assert (vertices (list_to_set ys ∪ g ∖ list_to_set xs) = vertices g) as Hvg.
-    { apply undo0_vertices in Hundo.
-      rewrite vertices_union Hundo -vertices_union -union_difference_L //.
+    { apply mirror_vertices in Hmirror.
+      rewrite vertices_union Hmirror -vertices_union -union_difference_L //.
       eauto using path_all_in. }
 
     constructor.
@@ -1501,22 +1386,23 @@ Section pstore_G.
       apply path_middle in Hpath. destruct Hpath as (y'&Hy'1&Hy'2).
       assert (y'=y) as ->.
       { inversion Hy'2; subst; inversion Hy2; naive_solver. }
-      edestruct use_undo as (zs&Hzs). eauto using undo0_undo_weak. done.
+      eapply use_mirror_subset in Hmirror. 3:apply Hy'1. 2:set_solver.
+      destruct Hmirror as (zs&Hzs&_).
       exists (ys1++zs). eapply path_app.
       2:{ eapply path_weak. done. set_solver. }
-      { clear X2. induction Hy1.
-        { apply path_nil. }
-        apply path_cons.
-        { rewrite elem_of_union elem_of_difference. right. split. set_solver.
-          apply not_elem_of_list_to_set.
-          eapply path_use_diff_last. 1,2: eauto using ti2.
-          3:{ apply diff_last_comm. done. }
-          { eapply path_app; eauto. }
-          { rewrite -app_comm_cons. eapply path_cons. done.
-            eapply path_app; eauto. }
-          { set_solver. } }
-        { apply IHHy1; eauto.  unfold diff_last in *. rewrite last_cons in Hlast.
-          destruct (last bs), (last ys2); try done. } } }
+      clear X2. induction Hy1.
+      { apply path_nil. }
+      apply path_cons.
+      { rewrite elem_of_union elem_of_difference. right. split. set_solver.
+        apply not_elem_of_list_to_set.
+        eapply path_use_diff_last. 1,2: eauto using ti2.
+        3:{ apply diff_last_comm. done. }
+        { eapply path_app; eauto. }
+        { rewrite -app_comm_cons. eapply path_cons. done.
+          eapply path_app; eauto. }
+        { set_solver. } }
+      { apply IHHy1; eauto.  unfold diff_last in *. rewrite last_cons in Hlast.
+        destruct (last bs), (last ys2); try done. } }
     { intros a zs Hzs. rewrite comm_L in Hzs.
       apply path_union_inv in Hzs. destruct Hzs as [Hsz|Hsz].
       (* The cycle is only in g, easy. *)
@@ -1526,14 +1412,14 @@ Section pstore_G.
       exfalso. destruct Hsz as (a'&x&l1&l2&E1&Hx&E2&->).
 
       apply path_cannot_escape with (r:=rs) in E2; last first.
-      { eapply use_undo'; eauto using undo_undo0. }
+      { eapply path_pathlike. eapply use_mirror; eauto. }
       { done. }
       { rewrite comm_L //. }
       { set_solver. }
 
       eapply path_weak in E1.
       eapply path_in_seg_complete with (r:=rs) in E1; last first. done.
-      { eapply use_undo'; eauto using undo_undo0. }
+      { eapply path_pathlike. eapply use_mirror; eauto. }
       { rewrite comm_L //. }
       { set_solver. }
       2:{ set_solver. }
@@ -1542,10 +1428,9 @@ Section pstore_G.
       assert (path (list_to_set ys) a (x0 ++ x::l2) a ) as Hcycle.
       { eapply path_app. done. done. }
 
-      eapply use_undo_weak' with (ys:=xs) in Hcycle.
-      2:{ apply undo0_symm in Hundo.
-          apply undo0_undo_weak in Hundo. apply path_all_in in Hcycle.
-          intros ????. eapply (Hundo _ x1); eauto. set_solver. }
+      eapply use_mirror_subset with (ys:=xs) in Hcycle.
+      3:{ by apply mirror_symm. }
+      2:{ apply path_all_in in Hcycle. set_solver. }
       destruct Hcycle as (?&Hcycle&F).
       eapply path_weak in Hcycle. 2:eapply path_all_in; done.
       eapply ti2 in Hcycle; eauto. subst. destruct x0; simpl in *; lia. }
@@ -1565,139 +1450,109 @@ Section pstore_G.
     { apply undo_cons. done. done. }
   Qed.
 
-  Lemma undo_app_inv1 xs ys1 ys2 σ :
-    undo xs (ys1 ++ ys2) σ ->
-    exists xs1 xs2, xs = xs2 ++ xs1 /\ undo xs1 ys1 σ.
-  Proof.
-    intros Hundo. apply undo_app_inv in Hundo. naive_solver.
-  Qed.
-
-  Lemma use_undo0 xs ys g r y :
-    undo0 xs ys ->
-    path g r xs y ->
-    path (list_to_set ys) y ys r.
-  Proof.
-    intros Hu. revert r y. induction Hu; intros r0 y.
-    { inversion 1. subst. apply path_nil. }
-    intros Hp. apply path_snoc_inv in Hp. destruct Hp as (?&?&?). subst.
-    apply path_cons. set_solver. eapply path_weak. apply IHHu; eauto. set_solver.
-  Qed.
-
-  Lemma same_path g (xs:list (loc* (loc*val)*loc)) a1 a2 a3 a4 :
+  Lemma construct_middlepoint (g:graph loc (loc*val)) a1 xs ys a2 a2' :
+    unaliased g ->
+    (forall x l', ¬ (a2,x,l') ∈ g) -> (* root has no succ *)
     path g a1 xs a2 ->
-    path g a3 xs a4 ->
-    xs ≠ nil ->
-    a1 = a3 /\ a2=a4.
+    path g a1 ys a2' ->
+    exists zs, xs = ys ++ zs.
   Proof.
-    intros Hp1. revert a3 a4. induction Hp1.
-    { intros. congruence. }
-    intros a3' a4'. inversion 1. subst. intros _. destruct bs.
-    { inversion Hp1; inversion H8. subst. done. }
-    apply IHHp1 in H8. 2:done. naive_solver.
+    intros Hinj Hroot Hpath. revert ys. induction Hpath; intros ys.
+    { intros Hpath. inversion Hpath. eauto. subst. set_solver. }
+    { intros X. inversion X; subst.
+      { exists ((a2', b, a2) :: bs ). done. }
+      destruct (Hinj _ _ _ _ _ H H0). subst.
+      apply IHHpath in H1. destruct H1 as (?&?).
+      eexists. rewrite -app_comm_cons H1 //.
+      intros ??. apply Hroot. }
   Qed.
 
-  Lemma undo_preserves_model g (M:map_model) (xs ys:list (loc* (loc*val)*loc)) (r1 r2:loc) ds σ1 σ2 rs σ0 σr r:
-     dom M = vertices g ∪ {[r]} ->
-    (forall r1 ds r2 σ1 σ2, reachable g r1 ds r2 -> M !! r1 = Some σ1 -> M !! r2 = Some σ2 -> σ1 ⊆ (apply_diffl ds σ2)) -> (* this is a part of _inv *)
+
+  Lemma undo_preserves_model g (M:map_model) (xs ys:list (loc* (loc*val)*loc)) rs σ0 r:
+    dom M = vertices g ∪ {[r]} ->
+    correct_path_diff M g ->
     (forall x l', ¬ (rs,x,l') ∈ (list_to_set ys ∪ g ∖ list_to_set xs)) -> (* root has no succ *)
-    kindofinj (g ∖ list_to_set xs ∪ list_to_set ys) ->
+    unaliased (g ∖ list_to_set xs ∪ list_to_set ys) ->
     path g rs xs r ->
     undo xs ys σ0 ->
-    reachable (list_to_set ys ∪ g ∖ list_to_set xs) r1 ds r2 ->
-    M !! r = Some σr -> σr ⊆ σ0 ->
-    M !! r1 = Some σ1 →
-    M !! r2 = Some σ2 →
-    σ1 ⊆ apply_diffl ds σ2.
+    M !! r = Some σ0 ->
+    correct_path_diff M (list_to_set ys ∪ g ∖ list_to_set xs).
   Proof.
-    intros Hdom Hinv Hroot Hinj' Hrs Hundo Hreach E0 R0 E1 E2. rewrite comm_L in Hreach.
-    apply reachable_path in Hreach. destruct Hreach as (zs&Hpath&<-).
+    intros Hdom Hinv Hroot Hinj' Hrs Hundo E0.
+    intros r1 zs r2 σ1 σ2 Hpath E1 E2. rewrite comm_L in Hpath.
     apply path_union_inv in Hpath. destruct Hpath as [Hpath|Hpath].
 
     (* If the path is entirely in g, easy. *)
-    { eapply Hinv; eauto. eapply reachable_path2. eapply path_weak. done. set_solver. }
+    { eapply Hinv; eauto. eapply path_weak. done. set_solver. }
+
+    assert (mirror xs ys) as Hmirror by eauto using undo_mirror.
 
     destruct Hpath as (a'&x&l1&l2&X1&Hx&X2&Hzs).
     eapply path_cannot_escape with (r:=rs) in X2; eauto; last first.
-    { eapply use_undo'; eauto using undo_undo0. }
+    { eapply path_pathlike. eapply use_mirror; eauto. }
     { set_solver. }
 
     (* otherwise the path includes a part in g, and a part in ys. *)
 
     assert (vertices (list_to_set ys ∪ g ∖ list_to_set xs) = vertices g) as Hvg.
-    { apply undo_undo0, undo0_vertices in Hundo.
-      rewrite vertices_union Hundo -vertices_union -union_difference_L //.
+    { apply mirror_vertices in Hmirror.
+      rewrite vertices_union Hmirror -vertices_union -union_difference_L //.
       eauto using path_all_in. }
 
     assert (a' ∈ dom M) as Ha'.
     { rewrite Hdom -Hvg elem_of_union. left. apply elem_of_vertices.
       inversion X2. set_solver. }
     apply elem_of_dom in Ha'. destruct Ha' as (σ',Ea').
-    assert (σ1 ⊆ apply_diffl (proj2 <$> l1) σ').
-    { apply reachable_path2 in X1.
-      eapply reachable_weak in X1.
+    assert (σ1 = (apply_diffl (proj2 <$> l1) σ')).
+    { eapply path_weak in X1.
       eapply (Hinv _ _ _ _ _ X1 E1 Ea'). set_solver. }
 
     (* The part in g is preserved. *)
+
     etrans. done. rewrite Hzs. rewrite fmap_app apply_diffl_app.
-    apply apply_diffl_included. clear dependent σ1 l1.
+    f_equal. clear dependent σ1 l1.
 
+    (* XXX facto a lemma. *)
     assert (exists u1 u2, ys = u1 ++ (x::l2) ++ u2) as (u1&u2&Hys).
-    { admit. }
+    { eapply use_mirror in Hrs. 2:done.
+      apply elem_of_list_to_set, elem_of_middle in Hx.
+      destruct Hx as (p1&p2&->).
+      apply path_app_inv in Hrs. destruct Hrs as (?&Hp1&Hp2).
+      inversion Hp2; inversion X2. subst. inversion H5. subst.
+      eapply construct_middlepoint in H10. 4:apply H4.
+      2:{ intros z1 z2 z3 z4 z5 ??. eapply (Hinj' z1 z2 z3 z4 z5); try done.
+          all:apply elem_of_union; right. all:set_solver. }
+      2:{ intros x l' X. eapply (Hroot x l').
+          apply elem_of_union. left. set_solver. }
+      destruct H10.
+      eexists _,_. f_equal. rewrite -app_comm_cons. f_equal. done. }
 
-    generalize Hundo. intros Hpath.
     rewrite Hys assoc_L in Hundo. apply undo_app_inv in Hundo.
     destruct Hundo as (xs1&xs2&->&Hundo1&Hundo2).
     apply undo_app_inv in Hundo2.
     destruct Hundo2 as (xs4&xs3&->&Hundo2&Hundo3).
 
-    eapply undo_undo0,use_undo0 in Hpath. 2:done.
-    rewrite {2}Hys in Hpath.
-    apply path_app_inv in Hpath. destruct Hpath as (n1&T1&T2).
+    eapply use_mirror in Hmirror. 2:done.
+    rewrite {2}Hys in Hmirror.
+    apply path_app_inv in Hmirror. destruct Hmirror as (n1&T1&T2).
     apply path_app_inv in T2. destruct T2 as (n2&T2&T3).
     edestruct (same_path (list_to_set ys) (x::l2) n1 n2 a') as (?&?); try done.
     subst n1 n2.
 
-    assert (reachable g a' (proj2 <$> xs4) r) as R1.
-    { apply reachable_path2. eapply path_weak.
-      eapply use_undo0. eapply undo0_symm,undo_undo0. done. done.
+    assert (path g a' xs4 r) as R1.
+    { eapply path_weak.
+      eapply use_mirror. eapply mirror_symm. eauto using undo_mirror. done.
       apply path_all_in in Hrs. set_solver. }
-    eapply Hinv in R1; try done.
+    apply (Hinv _ _ _ σ' σ0) in R1; try done.
 
-    assert (reachable g r2 (proj2 <$> xs3) a') as R2.
-    { apply reachable_path2. eapply path_weak.
-      eapply use_undo0. eapply undo0_symm,undo_undo0. done. done.
+    assert (path g r2 xs3 a') as R2.
+    { eapply path_weak.
+      eapply use_mirror. eapply mirror_symm. eauto using undo_mirror. done.
       apply path_all_in in Hrs. set_solver. }
-    eapply Hinv in R2; try done.
-    etrans. apply R1.
-
-    remember (apply_diffl (proj2 <$> xs4) σr) as μ.
-
-    Lemma undo_apply_diff xs ys σ σ' :
-    undo xs ys σ' ->
-    σ ⊆ apply_diffl (proj2 <$> ys) σ' ->
-    apply_diffl (proj2 <$> xs) σ ⊆ σ'.
-  Proof.
-    induction 1.
-    Abort.
-
-
-
-    Admitted.
-
-    path g a1 ys a2 ->
-         undo xs ys σ0
-
-    Search undo.
-
-    Search undo.
-
-    Search path.
-    }
-
-
-    Search undo.
+    eapply (Hinv _ _ _ σ2 σ') in R2; try done.
+    rewrite R2. rewrite -apply_diffl_app -fmap_app.
+    eapply use_undo. rewrite R1. done.
   Qed.
-
 
   Lemma pstore_restore_spec γ t σ s σ' :
     {{{
@@ -1715,7 +1570,7 @@ Section pstore_G.
     iDestruct "Hsnap" as "(%rs&%&->&Hsnap)".
     wp_rec. iStep 20.
 
-    iDestruct (extract_kindofinj with "Hg") as "%".
+    iDestruct (extract_unaliased with "Hg") as "%".
 
     iDestruct (map_agree_lookup with "[$][$]") as "%Hrs".
     apply Hsnap in Hrs. destruct Hrs as (σ1&HMrs&?).
@@ -1724,7 +1579,7 @@ Section pstore_G.
     { subst.
       subst.
       wp_load. iStep 9. iModIntro.
-      iExists _,_,_,_,_,_,_. iFrame. iPureIntro. split_and!; eauto.
+      iExists _,_,_,_,_,_. iFrame. iPureIntro. split_and!; eauto.
       { destruct Hinv as [X1 X2 X3 X4]. constructor; eauto. naive_solver. } }
 
     assert (rs ∈ vertices g) as Hrs.
@@ -1751,13 +1606,14 @@ Section pstore_G.
     { iFrame. }
 
     iIntros "[%ys (%Hundo&?&?&?)]".
+    assert (mirror xs ys) as Hmirror by eauto using undo_mirror.
     iStep 8. do 2 iModIntro.
     iApply "HΦ".
     iDestruct (big_sepS_union_2 with "[$][$]") as "Hs".
 
     remember ((rs, (l, v), r') :: bs) as xs.
 
-    iDestruct (extract_kindofinj with "Hs") as "%".
+    iDestruct (extract_unaliased with "Hs") as "%".
 
     assert (({[(rs, (l, v), r')]} ∪ list_to_set bs) = (list_to_set xs : gset _)) as Hbs.
     { subst xs. reflexivity. }
@@ -1765,38 +1621,37 @@ Section pstore_G.
 
     iAssert ⌜forall x y, (rs,x,y) ∉ (list_to_set ys ∪ g ∖ list_to_set xs)⌝%I as "%".
     { iIntros (???). destruct a. iDestruct (big_sepS_elem_of with "Hs") as "?". done.
-      iClear "H17".
-      iDestruct (mapsto_ne with "[$][$]") as "%". congruence. }
+      iDestruct (mapsto_ne rs rs with "[$][$]") as "%". congruence. }
 
-    iExists _,_,_,σ1,_,M,_. iFrame.
+    iExists _,_,_,_,M,_. iFrame.
 
     assert (vertices (list_to_set ys ∪ g ∖ list_to_set xs) = vertices g) as Hvg.
-    { apply undo_undo0, undo0_vertices in Hundo.
-      rewrite vertices_union Hundo -vertices_union -union_difference_L //. }
+    { apply mirror_vertices in Hmirror.
+      rewrite vertices_union Hmirror -vertices_union -union_difference_L //. }
 
-    assert (σ1 ⊆ apply_diffl (proj2 <$> xs) σ0).
-    { destruct Hinv as [X1 X2 X3 X4].
-      apply reachable_path2 in Hrs.
-      eapply X4 in Hrs. 2,3:done. etrans. apply Hrs.
-      destruct Hcoh. eauto using apply_diffl_included. }
+    assert (σ1 = (apply_diffl (proj2 <$> xs) σ0)).
+    { destruct Hinv as [X1 X2 X3 X4]. eauto. }
 
     assert (rooted_dag (list_to_set ys ∪ g ∖ list_to_set xs) rs) as Hroot.
-    { eapply undo_preserves_rooted_dag; eauto using undo_undo0. }
+    { eapply undo_preserves_rooted_dag; eauto. }
 
     iPureIntro. split_and !; try done.
     { destruct Hinv as [X1 X2 X3 X4]. constructor.
       { rewrite X1 Hvg.
         apply elem_of_dom_2 in X3,HMrs.
-        apply reachable_path2,reachable_inv_in_invertices in Hrs.
+        apply path_ends_vertices in Hrs.
         set_solver. }
-      { by etrans. }
-      { done. }
+      { subst xs. set_solver. }
+      { set_solver. }
       { intros. eapply undo_preserves_model; eauto. rewrite comm_L //. } }
-    { destruct Hcoh as [X1 X2]. constructor.
-      { subst xs. simpl in *. done. }
-      { replace (<[l:=v]> (foldr (λ '(l0, v0) σ2, <[l0:=v0]> σ2) σ0 (proj2 <$> bs))) with (apply_diffl (proj2 <$> xs) σ0).
-        2:{ subst xs. reflexivity. }
-        rewrite dom_apply_diffl. intros ???? Hedge.
+    { replace (<[l:=v]> (foldr (λ '(l0, v0) σ2, <[l0:=v0]> σ2) σ0 (proj2 <$> bs))) with (apply_diffl (proj2 <$> xs) σ0).
+      2:{ subst xs. reflexivity. }
+
+      destruct Hcoh as [X1 X2]. constructor.
+      { intros ???. rewrite dom_apply_diffl. apply X1 in H8.
+        eapply use_locs_of_edges_in in Hrs. 2:done.
+        set_solver. }
+      { rewrite dom_apply_diffl. intros ???? Hedge.
         rewrite /edge elem_of_union in Hedge. rewrite elem_of_union.
         destruct Hedge as [Hedge|Hedge].
         { right. eauto using undo_same_fst_label. }
